code/experimental/rsapss/Hacl.Impl.Bignum.Gcd.fst
@@ -1,0 +1,110 @@
+module Hacl.Impl.Bignum.Gcd
+
+open FStar.HyperStack.ST
+open FStar.HyperStack
+open FStar.Buffer
+open FStar.Mul
+
+open LowStar.Buffer
+
+open Lib.Buffer
+open Lib.IntTypes
+open Lib.Math.Algebra
+
+open Hacl.Impl.Bignum.Addition
+open Hacl.Impl.Bignum.Core
+open Hacl.Impl.Bignum.Comparison
+open Hacl.Impl.Bignum.Division
+open Hacl.Impl.Bignum.Misc
+open Hacl.Impl.Bignum.Multiplication
+open Hacl.Spec.Bignum
+
+
+val bn_gcd_:
+     #aLen:bn_len
+  -> a:lbignum aLen
+  -> b:lbignum aLen
+  -> g:lbignum aLen
+  -> tmp_q:lbignum aLen
+  -> tmp_r:lbignum aLen
+  -> Stack unit
+    (requires fun h ->
+     live h a /\ live h b /\ live h g /\ live h tmp_q /\ live h tmp_r /\
+     all_disjoint [loc a; loc b; loc g; loc tmp_q; loc tmp_r] /\
+     as_snat h b <> 0)
+    (ensures fun h0 _ h1 ->
+     modifies (loc a |+| loc b |+| loc g |+| loc tmp_q |+| loc tmp_r) h0 h1 /\
+     as_snat h1 g > 0 /\
+     as_snat h1 g = gcd_standalone (as_snat h0 a) (as_snat h0 b) /\
+     is_gcd (as_snat h0 a) (as_snat h0 b) (as_snat h1 g)
+     )
+let rec bn_gcd_ #aLen a b g tmp_q tmp_r =
+  if bn_is_zero a
+  then bn_assign_bn g b
+  else begin
+    bn_divide b a tmp_q tmp_r;
+    bn_assign_bn b tmp_r;
+    bn_gcd_ b a g tmp_q tmp_r
+  end
+
+
+#reset-options "--z3rlimit 50 --max_fuel 0 --max_ifuel 0"
+
+val bn_gcd:
+     #aLen:bn_len
+  -> a:lbignum aLen
+  -> b:lbignum aLen
+  -> g:lbignum aLen
+  -> Stack unit
+    (requires fun h ->
+      live h a /\ live h b /\ live h g /\
+      all_disjoint [loc a; loc b; loc g] /\
+      as_snat h b <> 0)
+    (ensures fun h0 _ h1 ->
+      modifies1 g h0 h1 /\
+      as_snat h1 g > 0 /\
+      as_snat h1 g = gcd_standalone (as_snat h0 a) (as_snat h0 b) /\
+      is_gcd (as_snat h0 a) (as_snat h0 b) (as_snat h1 g))
+let bn_gcd #aLen a b g =
+  push_frame ();
+  let a' = bn_copy a in
+  let b' = bn_copy b in
+  let tmp_q = create aLen (u64 0) in
+  let tmp_r = create aLen (u64 0) in
+  bn_gcd_ a' b' g tmp_q tmp_r;
+  pop_frame ()
+
+val bn_lcm:
+     #nLen:bn_len{v nLen * 2 < max_size_t}
+  -> a:lbignum nLen
+  -> b:lbignum nLen
+  -> l:lbignum nLen
+  -> Stack unit
+    (requires fun h ->
+      live h a /\ live h b /\ live h l /\
+      all_disjoint [loc a; loc b; loc l] /\
+      as_snat h a > 0 /\
+      as_snat h b > 0 /\
+      issnat (as_snat h a * as_snat h b) /\
+      v (nat_bytes_num (as_snat h a * as_snat h b)) <= v nLen
+      )
+    (ensures fun h0 _ h1 ->
+      modifies1 l h0 h1 /\
+      as_snat h1 l > 0 /\
+      as_snat h1 l = lcm (as_snat h0 a) (as_snat h0 b))
+let bn_lcm #nLen a b l =
+  push_frame ();
+  let g = create nLen (u64 0) in
+  bn_gcd a b g;
+  let tmp = create nLen (u64 0) in
+  let tmp_unused = create nLen (u64 0) in
+  bn_divide a g tmp tmp_unused;
+
+  let h = FStar.HyperStack.ST.get () in
+  division_post_size (as_snat h a) (as_snat h g);
+  snat_order (as_snat h tmp * as_snat h b) (as_snat h a * as_snat h b);
+  nat_bytes_num_fit (as_snat h tmp * as_snat h b) (as_snat h a * as_snat h b);
+
+  bn_mul_fitting tmp b l;
+
+  pop_frame ()
